Implement & prove fusion transformation

examples/Fusion.v
@@ -3,43 +3,12 @@ Require Import CUDALib Correctness.
 Require Import Compiler Ext Extract Host CompilerProof LibTactics.
 Open Scope Z_scope.
 
-Notation AVFusedEnv0 GA1 GA2 := (hlist (fun typ => option (Skel.Func GA2 (Skel.Fun1 Skel.TZ typ) * Skel.LExp GA2 Skel.TZ)) GA1).
+Notation AVFusedEnv0 GA1 GA2 := (hlist (fun typ => sum (member typ GA2) (Skel.Func GA2 (Skel.Fun1 Skel.TZ typ) * Skel.LExp GA2 Skel.TZ)) GA1).
 Notation AVFusedEnv GA := (AVFusedEnv0 GA GA).
 
 Axiom sorry : forall {T : Type}, T.
 
 Import Skel.
-
-Fixpoint shift_lexp_GA {GA resTy} ty (le : LExp GA resTy) : LExp (ty :: GA) resTy :=
-  match le in LExp _ resTy  return LExp (ty :: GA) resTy with
-  | LNum _ n => LNum _ n
-  | LMin _ le1 le2 => LMin _ (shift_lexp_GA _ le1) (shift_lexp_GA _ le2)
-  | LLen _ t m => LLen _ t (HNext m)
-  end.
-
-Lemma shift_lexp_GA_ok GA resTy ty (le : LExp GA resTy) :
-  forall arr aeenv,
-    lexpDenote _ _ (shift_lexp_GA ty le) (arr ::: aeenv) =
-    lexpDenote _ _ le aeenv.
-Proof.
-  dependent induction le; simpl; introv; eauto.
-  rewrites* IHle1; rewrites* IHle2.
-Qed.
-
-Definition shift_fused_env {GA typ} (avfenv : AVFusedEnv0 (typ :: GA) GA) : AVFusedEnv (typ :: GA) :=
-  hmap (fun typ' darr =>
-    match darr with
-    | None => None
-    | Some (f, lexp) => Some (shift_func_GA typ f, shift_lexp_GA typ lexp)
-    end) avfenv.
-
-Definition body_of_func1 {GA ty1 ty2} (f : Func GA (Fun1 ty1 ty2)) : SExp GA [ty1] ty2 :=
-  match f in Func _ fty return (match fty with
-                                | Fun1 ty1 ty2 => SExp _ [ty1] ty2
-                                | Fun2 _ _ _ =>  unit end) with
-  | F1 _ _ _ body => body
-  | _ => tt
-  end.
 
 Fixpoint insertAt {T} (t : T) (G : list T) (n : nat) {struct n} : list T :=
   match n with
@@ -60,6 +29,12 @@ Fixpoint liftVar {A} {t : A} {G} (x : member t G) t' n : member t (insertAt t' G
                            | O => HNext (HNext x')
                            | S n' => HNext (liftVar x' t' n')
                          end
+  end.
+
+Fixpoint liftVar_many {A} {t : A} {G} (x : member t G) G' : member t (G ++ G') :=
+  match x with
+  | HFirst => HFirst
+  | @HNext _ _ t'' G' x' => HNext (liftVar_many x' _)
   end.
 
 Fixpoint insertAtS {A ls f} (t : A) (x : f t) (n : nat) {struct n}
@@ -87,6 +62,20 @@ Fixpoint lift_sexp {GA GS} {resTy} ty (se : SExp GA GS resTy) n : SExp GA (inser
   | ELet _ _ _ _ e1 e2 => ELet _ _ _ _ (lift_sexp ty e1 n) (lift_sexp ty e2 (S n))
   end.
 
+Fixpoint lift_many_sexp {GA GS} {resTy} (se : SExp GA GS resTy) GS' : SExp GA (GS ++ GS') resTy :=
+  match se with
+  | ENum n => ENum n
+  | EVar _ _ _ m => EVar _ _ _ (liftVar_many m GS')
+  | EBin _ _ _ _ _ op e1 e2 => EBin _ _ _ _ _ op (lift_many_sexp e1 GS') (lift_many_sexp e2 GS')
+  | EA _ _ _ m se => EA _ _ _ m (lift_many_sexp se GS')
+  | ELen _ _ _ m => ELen _ _ _ m
+  | EIf _ _ _ e1 e2 e3 => EIf _ _ _ (lift_many_sexp e1 GS') (lift_many_sexp e2 GS') (lift_many_sexp e3 GS')
+  | ECons _ _ _ _ e1 e2 => ECons _ _ _ _ (lift_many_sexp e1 GS') (lift_many_sexp e2 GS')
+  | EPrj1 _ _ _ _ e => EPrj1 _ _ _ _ (lift_many_sexp e GS')
+  | EPrj2 _ _ _ _ e => EPrj2 _ _ _ _ (lift_many_sexp e GS')
+  | ELet _ _ _ _ e1 e2 => ELet _ _ _ _ (lift_many_sexp e1 GS') (lift_many_sexp e2 GS')
+  end.
+
 Lemma insertAtS_liftVar A ls f (hls : hlist f ls) (t : A)(m : member t ls) v (x : f v) :
   forall n,
     hget (insertAtS v x n hls) (liftVar m v n) =
@@ -110,6 +99,58 @@ Proof.
   2:forwards*: (>>IHse2 aeenv (t ::: seenv) ty v (S n)).
   rewrites* insertAtS_liftVar.
 Qed.  
+
+Lemma liftVar_many_ok A (ls : list A) f (hls : hlist f ls) t (m : member t ls) :
+  forall ls' hls',
+    hget hls m = hget (hls +++ hls') (liftVar_many m ls').
+Proof.
+  dependent induction hls; dependent destruction m; simpl; eauto.
+Qed.
+    
+Lemma lift_many_sexp_ok GA GS resTy (se : SExp GA GS resTy) :
+  forall aeenv GS' seenv seenv', 
+    sexpDenote (lift_many_sexp se GS') aeenv (seenv +++ seenv') = sexpDenote se aeenv seenv.
+Proof.
+  induction se; simpl; intros;
+    unfold ret, bind; simpl; unfold bind_opt;
+      (try rewrites* IHse); (try rewrites* IHse1); (try rewrites* IHse2);
+        (try rewrites* IHse3); jauto.
+  rewrites* <-(>>liftVar_many_ok).
+  destruct sexpDenote; jauto.
+  forwards*: (>>IHse2 (t ::: seenv)).
+Qed.  
+
+Fixpoint shift_lexp_GA {GA resTy} ty (le : LExp GA resTy) : LExp (ty :: GA) resTy :=
+  match le in LExp _ resTy  return LExp (ty :: GA) resTy with
+  | LNum _ n => LNum _ n
+  | LMin _ le1 le2 => LMin _ (shift_lexp_GA _ le1) (shift_lexp_GA _ le2)
+  | LLen _ t m => LLen _ t (HNext m)
+  end.
+
+Lemma shift_lexp_GA_ok GA resTy ty (le : LExp GA resTy) :
+  forall arr aeenv,
+    lexpDenote _ _ (shift_lexp_GA ty le) (arr ::: aeenv) =
+    lexpDenote _ _ le aeenv.
+Proof.
+  dependent induction le; simpl; introv; eauto.
+  rewrites* IHle1; rewrites* IHle2.
+Qed.
+
+Definition shift_fused_env {GA GA' typ} (avfenv : AVFusedEnv0 GA GA') : AVFusedEnv0 GA (typ :: GA') :=
+  hmap (fun typ' darr =>
+    match darr with
+    | inl m => inl (liftVar m typ 0)
+    | inr (f, lexp) => inr (shift_func_GA typ f, shift_lexp_GA typ lexp)
+    end) avfenv.
+
+Definition body_of_func1 {GA ty1 ty2} (f : Func GA (Fun1 ty1 ty2)) : SExp GA [ty1] ty2 :=
+  match f in Func _ fty return (match fty with
+                                | Fun1 ty1 ty2 => SExp _ [ty1] ty2
+                                | Fun2 _ _ _ =>  unit end) with
+  | F1 _ _ _ body => body
+  | _ => tt
+  end.
+
 
 Definition fuse_f1 {GA ty1 ty2 ty3}
   (f : Func GA (Fun1 ty1 ty2)) (g : Func GA (Fun1 ty2 ty3)) : Func GA (Fun1 ty1 ty3) :=
@@ -135,48 +176,212 @@ Definition darr_of_skelapp {GA resTy}  (skel : SkelE GA resTy) :
     Some (Skel.F1 _ _ _ (Skel.ECons _ _ _ _ body1 body2), Skel.LMin _ len1 len2)
   end.
 
-Definition fuse_ae {GA resTy} (ae : AE GA resTy) : AVFusedEnv GA -> AE GA resTy :=
+Fixpoint fuse_se {GA GA' GS resTy} (se : SExp GA GS resTy) : AVFusedEnv0 GA GA' -> SExp GA' GS resTy :=
+  match se with
+  | ENum n => fun avfenv => ENum n
+  | EVar _ _ _ m => fun avfenv =>  EVar _ _ _ m
+  | EBin _ _ _ _ _ op e1 e2 =>
+    fun avfenv => EBin _ _ _ _ _ op (fuse_se e1 avfenv) (fuse_se e2 avfenv)
+  | EA _ _ _ m se =>
+    fun avfenv =>
+      let se := fuse_se se avfenv in
+      match hget avfenv m with
+      | inl m => EA _ _ _ m se
+      | inr (f, len) =>
+        let body := body_of_func1 f in
+        ELet _ _ _ _ se (lift_many_sexp body _)
+      end
+  | ELen _ _ _ m =>
+    fun avfenv =>
+      match hget avfenv m with
+      | inl m => ELen _ _ _ m
+      | inr (f, len) => lexp2sexp _ _ len _
+      end
+  | EIf _ _ _ e1 e2 e3 =>
+    fun avfenv =>
+      EIf _ _ _ (fuse_se e1 avfenv) (fuse_se e2 avfenv) (fuse_se e3 avfenv)
+  | ECons _ _ _ _ e1 e2 =>
+    fun avfenv =>
+      ECons _ _ _ _ (fuse_se e1 avfenv) (fuse_se e2 avfenv) 
+  | EPrj1 _ _ _ _ e =>
+    fun avfenv => EPrj1 _ _ _ _ (fuse_se e avfenv)
+  | EPrj2 _ _ _ _ e =>
+    fun avfenv => EPrj2 _ _ _ _ (fuse_se e avfenv)
+  | ELet _ _ _ _ e1 e2 =>
+    fun avfenv => ELet _ _ _ _ (fuse_se e1 avfenv) (fuse_se e2 avfenv) 
+  end.
+
+Definition fuse_func {GA GA' fty} (func : Func GA fty) : AVFusedEnv0 GA GA' -> Func GA' fty :=
+  match func with
+  | F1 _ _ _ se => fun avfenv => F1 _ _ _ (fuse_se se avfenv)
+  | F2 _ _ _ _ se => fun avfenv => F2 _ _ _ _ (fuse_se se avfenv)
+  end.
+
+Fixpoint fuse_le {GA GA' resTy} (le : LExp GA resTy) : AVFusedEnv0 GA GA' -> LExp GA' resTy :=
+  match le with
+  | LNum _ n => fun _ => LNum _ n
+  | LLen _ _ m =>
+    fun avfenv =>
+      match hget avfenv m with
+      | inl m => LLen _ _ m
+      | inr (f, l) => l
+      end
+  | LMin _ l1 l2 =>
+    fun avfenv =>
+      LMin _ (fuse_le l1 avfenv) (fuse_le l2 avfenv)
+  end.
+
+Definition fuse_ae {GA GA' resTy} (ae : AE GA resTy) : AVFusedEnv0 GA GA' -> AE GA' resTy :=
   match ae with
   | VArr _ _ m =>
     fun avfenv =>
       match hget avfenv m with
-      | None => VArr _ _ m
-      | Some (f, len) => DArr _ _ f len
+      | inl m => VArr _ _ m
+      | inr (f, len) => DArr _ _ f len
       end
   | DArr _ _ f l =>
-    fun avfenv => DArr _ _ f l
+    fun avfenv => DArr _ _ (fuse_func f avfenv) (fuse_le l avfenv)
   end.
 
-Definition fuse_skel {GA resTy} (skel : SkelE GA resTy) : AVFusedEnv GA -> SkelE GA resTy :=
+Definition fuse_skel {GA GA' resTy} (skel : SkelE GA resTy) : AVFusedEnv0 GA GA' -> SkelE GA' resTy :=
   match skel with
-  | Reduce _ _ f ae => fun avfenv => Reduce _ _ f (fuse_ae ae avfenv)
-  | Map _ _ _ f ae => fun avfenv => Map _ _ _ f (fuse_ae ae avfenv)
-  | Seq _ n l => fun _ => Seq _ n l
+  | Reduce _ _ f ae => fun avfenv => Reduce _ _ (fuse_func f avfenv) (fuse_ae ae avfenv)
+  | Map _ _ _ f ae => fun avfenv => Map _ _ _ (fuse_func f avfenv) (fuse_ae ae avfenv)
+  | Seq _ n l => fun avfenv => Seq _ (fuse_le n avfenv) (fuse_le l avfenv)
   | Zip _ _ _ ae1 ae2 => fun avfenv => Zip _ _ _ (fuse_ae ae1 avfenv) (fuse_ae ae2 avfenv)
   end.
 
-Fixpoint simple_fusion {GA typ} (p : AS GA typ) : AVFusedEnv GA -> AS GA typ :=
+Fixpoint simple_fusion {GA GA' typ} (p : AS GA typ) : AVFusedEnv0 GA GA' -> AS GA' typ :=
   match p with
   | ALet _ tyapp tyres skel res =>
     fun avfenv =>
       let skel := fuse_skel skel avfenv in
-      let darr := darr_of_skelapp skel in
-      let res := simple_fusion res (shift_fused_env (darr ::: avfenv)) in
-      ALet _ tyapp tyres skel res
+      if true then
+        match darr_of_skelapp skel with
+        | Some darr => simple_fusion res (inr darr ::: avfenv)
+        | None => ALet _ _ _ skel (simple_fusion res (inl HFirst ::: shift_fused_env avfenv))
+        end
+      else
+        ALet _ _ _ skel (simple_fusion res (inl HFirst ::: shift_fused_env avfenv))
   | ARet _ t x =>
     fun avfenv =>
-      ARet _ t x
+      match hget avfenv x with
+      | inl m => ARet _ _ m
+      | inr (f, l) =>
+        ALet _ _ _ (Map _ _ _ (F1 _ _ _ (EVar _ _ _ HFirst)) (DArr _ _ f l))
+             (ARet _ _ HFirst)
+      end
   end.
 
-Lemma fuse_ae_correct GA typ (ae : AE GA typ) :
-  forall (avfenv : AVFusedEnv GA) (aeenv : AEvalEnv GA),
-    (forall (m : member typ GA) f le,
-        hget avfenv m = Some (f, le)
-        -> aeDenote _ _ (DArr _ _ f le) aeenv = ret (hget aeenv m))
-    -> aeDenote _ _ (fuse_ae ae avfenv) aeenv = aeDenote _ _ ae aeenv.
+Lemma fuse_le_correct GA GA' typ (le : LExp GA typ) :
+  forall (avfenv : AVFusedEnv0 GA GA') (aeenv : AEvalEnv GA) (aeenv' : AEvalEnv GA'),
+    (forall ty (m : member ty GA) m',
+        hget avfenv m = inl m' -> hget aeenv' m' = hget aeenv m)
+    -> (forall ty (m : member ty GA) f le,
+           hget avfenv m = inr (f, le) ->
+           aeDenote _ _ (DArr _ _ f le) aeenv' = ret (hget aeenv m))
+    -> lexpDenote _ _ (fuse_le le avfenv) aeenv' = lexpDenote _ _ le aeenv.
 Proof.
-  destruct ae; simpl; introv; eauto.
-  destruct (hget avfenv m) as [[f le] | ] eqn:Heq; eauto.
+  induction le; introv Henv1 Henv2; simpl; eauto.
+  - destruct (hget avfenv m) as [|[? ?]]eqn:Heq;
+      [forwards*: Henv1; simpl; congruence|].
+    forwards*: Henv2; simpl in *.
+    destruct Z_le_dec; [|inverts H].
+    rewrites* (>>mapM_length H); rewrite seq_length, Z2Nat.id; eauto.
+  - rewrites* (>>IHle1 Henv1 Henv2).
+    rewrites* (>>IHle2 Henv1 Henv2).
+Qed.
+
+Lemma fuse_sexp_correct GA GA' GS typ (se : SExp GA GS typ) :
+  forall (avfenv : AVFusedEnv0 GA GA') (seenv : SEvalEnv GS) (aeenv : AEvalEnv GA) (aeenv' : AEvalEnv GA'),
+    (forall ty (m : member ty GA) m',
+        hget avfenv m = inl m' -> hget aeenv' m' = hget aeenv m)
+    -> (forall ty (m : member ty GA) f le,
+           hget avfenv m = inr (f, le) ->
+           aeDenote _ _ (DArr _ _ f le) aeenv' = ret (hget aeenv m))
+    -> forall res, sexpDenote se aeenv seenv = Some res
+    -> sexpDenote (fuse_se se avfenv) aeenv' seenv = Some res.
+Proof.
+  induction se; introv Henv1 Henv2; simpl in *; eauto.
+  all: unfold ret, bind; simpl; unfold bind_opt; introv Heq;
+    (repeat let Hfv := fresh in
+           match type of Heq with
+           | context [match sexpDenote ?se ?aeenv ?seenv with Some _ => _ | None => _ end] => destruct (sexpDenote se aeenv seenv) as [?|] eqn:Hfv; [|inverts Hfv; try congruence] end); inverts Heq;
+    try now(try rewrites* (>>IHse seenv Henv1 Henv2);
+            try rewrites* (>>IHse1 seenv Henv1 Henv2);
+            try rewrites* (>>IHse2 seenv Henv1 Henv2);
+            try rewrites* (>>IHse3 seenv Henv1 Henv2)).
+  - destruct (hget avfenv m) as [|[f l]] eqn:Henv;
+    simpl; unfold bind, ret; simpl; unfold bind_opt.
+    + rewrites* (>>IHse); rewrites* (>>Henv1).
+    + rewrites* (>>IHse); destruct sexpDenote; [|congruence].
+      forwards*: (>>Henv2).
+      dependent destruction f; simpl in *.
+      rewrites* (>>lift_many_sexp_ok ((t0 : typDenote TZ) ::: HNil) seenv).
+      destruct Z_le_dec; [|unfold ret in *; simpl in *; congruence].
+      forwards*HeqLen: (>>mapM_length).
+      forwards*Hval: (>>mapM_some (Z.to_nat t0) (0 : typDenote TZ) (@defval' t) H0).
+      rewrite seq_length in *.
+      rewrite <-HeqLen in Hval.
+      forwards*(? & ? & ?): (>>SeqCompiler.nth_error_lt_nat); substs.
+      rewrites Nat2Z.id in *; destruct lt_dec; try omega.
+      rewrite seq_nth in Hval; rewrite <-HeqLen in Hval; destruct lt_dec; try omega.
+      rewrite Z.add_0_l in Hval; rewrite <-Hval.
+      rewrites (>>nth_error_some' (@defval' t)); try omega.
+      rewrite Nat2Z.id; eauto.
+  - destruct (hget avfenv m) as [|[f l]] eqn:Henv;
+    simpl; unfold bind, ret; simpl; unfold bind_opt.
+    + rewrites* (>>Henv1).
+    + forwards*: (>>Henv2).
+      rewrite lexp2sexp_ok.
+      destruct Z_le_dec; [|unfold ret in *; inverts H].
+      forwards*Hlen: mapM_length.
+      rewrite seq_length in Hlen; rewrite Hlen, Z2Nat.id; eauto.
+  - rewrites* (>>IHse1 seenv Henv1 Henv2 H).
+    destruct t0; [rewrites* (>>IHse2 seenv Henv1 Henv2 H1)|rewrites* (>>IHse3 seenv Henv1 Henv2 H1)].
+  - rewrites* (>>IHse1 seenv Henv1 Henv2 H).
+    rewrites* (>>IHse2 (t ::: seenv) Henv1 Henv2 H1).
+Qed.
+
+Lemma mapM_eq A B (f g : A -> option B) ls :
+  (forall x, List.In x ls -> f x = g x)
+  -> mapM f ls = mapM g ls.
+Proof.
+  induction ls; simpl; eauto.
+  intros.
+  unfold mapM in *; simpl; unfold ret, bind; simpl; unfold bind_opt.
+  rewrite H; eauto.
+  destruct g; eauto.
+  rewrite IHls; eauto.
+Qed.
+
+Lemma fuse_ae_correct GA GA' typ (ae : AE GA typ) :
+  forall (avfenv : AVFusedEnv0 GA GA') (aeenv : AEvalEnv GA) (aeenv' : AEvalEnv GA'),
+    (forall ty (m : member ty GA) m',
+        hget avfenv m = inl m' -> hget aeenv' m' = hget aeenv m)
+    -> (forall ty (m : member ty GA) f le,
+           hget avfenv m = inr (f, le) -> aeDenote _ _ (DArr _ _ f le) aeenv' = ret (hget aeenv m))
+    -> forall res,
+        aeDenote _ _ ae aeenv = Some res
+        -> aeDenote _ _ (fuse_ae ae avfenv) aeenv' = Some res.
+Proof.
+  destruct ae; simpl; introv Henv1 Henv2 Hres; eauto.
+  - destruct (hget avfenv m) as [m' | [f le] ] eqn:Heq; simpl in *.
+    + forwards*: (>>Henv1); congruence.
+    + forwards*: (>>Henv2); congruence.
+  - rewrites* (>>fuse_le_correct).
+    destruct Z_le_dec; eauto.
+    dependent destruction f; simpl in *.
+    rewrite <- Hres.
+    apply mapM_eq; intros i H.
+    unfold seq in H; apply seq'_In in H.
+    forwards*: (>>mapM_some (Z.to_nat i) i (@defval' cod) Hres).
+    rewrite seq_length, Z2Nat.id in *; try omega.
+    destruct lt_dec; try omega.
+    2: rewrite <-Z2Nat.inj_lt in *; try omega.
+    rewrite seq_nth in H0; destruct lt_dec; try omega.
+    rewrite Z.add_0_l, Z2Nat.id in *; try omega.
+    rewrites* (>>fuse_sexp_correct).
 Qed.
 
 Lemma shift_sexp_GA_ok GA GS resTy ty (se : SExp GA GS resTy) :
@@ -192,16 +397,54 @@ Proof.
   destruct (Skel.sexpDenote se1 _ _); eauto.
   destruct t0; eauto.
 Qed.    
-  
-Lemma fuse_skel_correct GA resTyp (skel : SkelE GA resTyp) :
-  forall (avfenv : AVFusedEnv GA) (aeenv : AEvalEnv GA),
-    (forall typ (m : member typ GA) f le,
-        hget avfenv m = Some (f, le)
-        -> aeDenote _ _ (DArr _ _ f le) aeenv = ret (hget aeenv m))
-    -> skelDenote _ _ (fuse_skel skel avfenv) aeenv = skelDenote _ _ skel aeenv.
+
+Lemma mapM_some_in A B ls :forall ls' (f : A -> option B) x,
+  mapM f ls = Some ls'
+  -> List.In x ls
+  -> exists y, f x = Some y.
 Proof.
-  dependent destruction skel; simpl; eauto; introv Henv;
-    repeat rewrites* fuse_ae_correct.
+  induction ls; simpl; try tauto.
+  unfold mapM in *; simpl; unfold ret, bind; simpl; unfold bind_opt.
+  introv H HeqHin; substs.
+  destruct (f a) eqn:Heq; [|inverts H].
+  destruct HeqHin; substs.
+  - exists b; eauto.
+  - destruct sequence eqn:Heq'; inverts H.
+    forwards*: IHls.
+Qed.
+
+Lemma fuse_skel_correct GA GA' resTyp (skel : SkelE GA resTyp) :
+  forall (avfenv : AVFusedEnv0 GA GA') (aeenv : AEvalEnv GA) (aeenv' : AEvalEnv GA'),
+    (forall ty (m : member ty GA) m',
+        hget avfenv m = inl m' -> hget aeenv' m' = hget aeenv m)
+    -> (forall ty (m : member ty GA) f le,
+           hget avfenv m = inr (f, le) ->
+           aeDenote _ _ (DArr _ _ f le) aeenv' = ret (hget aeenv m))
+    -> skelE_wf _ _ skel
+    -> forall res,
+        skelDenote _ _ skel aeenv = Some res
+        -> skelDenote _ _ (fuse_skel skel avfenv) aeenv' = Some res.
+Proof.
+  dependent destruction skel; simpl; eauto; introv Henv1 Henv2 Hwf;
+    unfold ret, bind; simpl; unfold bind_opt;
+  intros res Hres.
+  - dependent destruction f; simpl.
+    destruct aeDenote eqn:heq; inversion Hres.
+    rewrites* (>>fuse_ae_correct).
+    apply mapM_eq; intros i Hin.
+    forwards*(? & ?): mapM_some_in.
+    rewrites* (>>fuse_sexp_correct).
+  - destruct aeDenote eqn:heq; inversion Hres.
+    rewrites* (>>fuse_ae_correct).
+    f_equal.
+    inverts Hwf; substs.
+    dependent destruction f; simpl in *.
+    extensionality x; extensionality y.
+    rewrites* (>>fuse_sexp_correct).
+  - repeat rewrites* (>>fuse_le_correct).
+  - destruct aeDenote eqn:heq; [|inversion Hres].
+    destruct (aeDenote GA t2) eqn:heq'; inverts Hres.
+    repeat rewrites* (>>fuse_ae_correct).
 Qed.  
 
 Lemma darr_of_skelapp_ok GA resTy (skel : SkelE GA resTy) :
@@ -313,42 +556,68 @@ Proof.
         unfold ret in Heq3; simpl in Heq3; congruence.
 Qed.
 
-Lemma simple_fusion_correct GA typ (p : AS GA typ) :
-  forall (avfenv : AVFusedEnv GA) (aeenv : AEvalEnv GA),
-    (forall typ (m : member typ GA) f le,
-        hget avfenv m = Some (f, le)
-        -> aeDenote _ _ (DArr _ _ f le) aeenv = ret (hget aeenv m))
-    -> forall res, 
+Lemma simple_fusion_correct GA typ (p : AS GA typ) : forall GA',
+  forall (avfenv : AVFusedEnv0 GA GA') (aeenv : AEvalEnv GA) (aeenv' : AEvalEnv GA'),
+    (forall ty (m : member ty GA) m',
+        hget avfenv m = inl m' -> hget aeenv' m' = hget aeenv m)
+    -> (forall ty (m : member ty GA) f le,
+           hget avfenv m = inr (f, le) ->
+           aeDenote _ _ (DArr _ _ f le) aeenv' = ret (hget aeenv m))
+    -> skel_as_wf _ _ p
+    -> forall res,
       asDenote _ _ p aeenv = Some res
-      -> asDenote _ _ (simple_fusion p avfenv) aeenv = Some res.
+      -> asDenote _ _ (simple_fusion p avfenv) aeenv' = Some res.
 Proof.
-  dependent induction p; simpl; eauto; introv Henv.
-  unfold bind, ret; simpl; unfold bind_opt; simpl.
-  rewrites* fuse_skel_correct.
-  destruct (skelDenote GA t1 s) eqn:Heq; eauto.
-  intros; forwards*: IHp.
-  introv Hget.
-  dependent destruction m; simpl in *.
-  - destruct darr_of_skelapp as [[f' le']|] eqn:Hdarr; inverts Hget.
-    rewrite shift_lexp_GA_ok.
-    forwards*Happ: darr_of_skelapp_ok.
-    rewrites* <-(>>fuse_skel_correct avfenv) in Heq.
-    simpl in *.
-    unfold ret; simpl; rewrite <-Happ.
-    destruct Z_le_dec; eauto.
-    f_equal; extensionality x.
-    dependent destruction f'; simpl.
-    rewrites* shift_sexp_GA_ok.
-  - rewrite hget_hmap in Hget.
-    destruct (hget avfenv m) as [[f' le']|] eqn:Heq'; inverts Hget.
-    rewrites* <-(>>Henv).
-    rewrites shift_lexp_GA_ok.
-    asserts_rewrite*
-    ((fun i : Z =>
-        funcDenote (t1 :: GA) (Fun1 TZ typ) (shift_func_GA t1 f') (a ::: aeenv) i) =
-     (fun i : Z => funcDenote GA (Fun1 TZ typ) f' aeenv i)).
-    extensionality i.
-    dependent destruction f'; simpl.
-    rewrites* shift_sexp_GA_ok.
+  dependent induction p; simpl; eauto; introv Henv1 Henv2 Hwf.
+  - unfold bind, ret; simpl; unfold bind_opt; simpl.
+    introv Heq.
+    destruct (skelDenote GA t1) eqn:Heq1; [|inverts Heq].
+    inverts Hwf.
+    destruct darr_of_skelapp as [[f' le']|] eqn:Hdarr; simpl.
+    + (* Can be fused to other funcs *)
+      intros; forwards*: IHp.
+      (* Prove invariant Henv1 & Henv2 is preserved *)
+      * intros.
+        dependent destruction m; simpl in *; jauto.
+        inverts H.
+      * intros.
+        dependent destruction m; simpl in *; jauto.
+        inverts H.
+        forwards*Happ: darr_of_skelapp_ok.
+        rewrites* <-(>>fuse_skel_correct Heq1).
+    + (* Cannot be fused *)
+      unfold bind, ret; simpl; unfold bind_opt.
+      rewrites* (>>fuse_skel_correct Heq1).
+      rewrites* (>>IHp).
+      * intros.
+        dependent destruction m; simpl in *; jauto.
+        inverts H; eauto.
+        dependent destruction m'; simpl in *; jauto.
+        unfold shift_fused_env in H; rewrite hget_hmap in H.
+        destruct (hget avfenv m) as [|[? ?]]; [|inverts H].
+        dependent destruction m0; inverts H.
+        forwards*: Henv1.
+        unfold shift_fused_env in H; rewrite hget_hmap in H.
+        destruct (hget avfenv m) as [|[? ?]] eqn:Henv; inverts H.
+        dependent destruction m0; simpl in *; inverts* H1.
+      * intros.
+        dependent destruction m; inverts H; simpl.
+        unfold shift_fused_env in *; rewrite hget_hmap in *.
+        destruct hget as [|[? ?]] eqn:?; inverts H1.
+        forwards*: Henv2.
+        rewrite shift_lexp_GA_ok.
+        rewrite <-H.
+        destruct Z_le_dec; eauto.
+        apply mapM_eq.
+        intros.
+        unfold seq in *; apply seq'_In in H0.
+        dependent destruction f0; simpl.
+        rewrites* shift_sexp_GA_ok.
+  - introv Hres; destruct (hget avfenv m) as [|[f' le']] eqn:Heq; eauto.
+    { simpl; rewrites* (>>Henv1). }
+    simpl; unfold bind, ret; simpl; unfold bind_opt.
+    rewrites* (>>Henv2).
+    rewrite Hres.
+    rewrite mapM_total.
+    rewrites* List.map_id.
 Qed.
-
